feat: sdk-integration

DynamoDbEncryptionMiddlewareInternal/src/AwsCryptographyDynamoDbEncryptionMiddlewareInternalOperations.dfy
@@ -1,19 +1,30 @@
 // Copyright Amazon.com Inc. or its affiliates. All Rights Reserved.
 // SPDX-License-Identifier: Apache-2.0
 include "../../private-aws-encryption-sdk-dafny-staging/ComAmazonawsDynamodb/Model/ComAmazonawsDynamodbTypes.dfy"
+include "../../private-aws-encryption-sdk-dafny-staging/libraries/src/Collections/Maps/Maps.dfy"
 include "../Model/AwsCryptographyDynamoDbEncryptionMiddlewareInternalTypes.dfy"
+include "../../StructuredEncryption/Model/AwsCryptographyStructuredEncryptionTypes.dfy"
+include "../../DynamoDbItemEncryptor/Model/AwsCryptographyDynamoDbItemEncryptorTypes.dfy"
+include "../../DynamoDbItemEncryptor/src/DynamoToStruct.dfy"
+include "DdbStatement.dfy"
 
 // TODO break this into multiple files
 module AwsCryptographyDynamoDbEncryptionMiddlewareInternalOperations refines AbstractAwsCryptographyDynamoDbEncryptionMiddlewareInternalOperations {
   import DDB = ComAmazonawsDynamodbTypes
   import AwsCryptographyDynamoDbItemEncryptorTypes
   import DynamoDbItemEncryptor
+  import DynamoToStruct
+  import ENC = AwsCryptographyDynamoDbItemEncryptorOperations
+  import EncTypes = AwsCryptographyDynamoDbItemEncryptorTypes
+  import AwsCryptographyStructuredEncryptionTypes
+  import Seq
+  import DdbStatement
 
   datatype TableConfig = TableConfig(
     partitionKeyName: string,
     sortKeyName: Option<string>,
     itemEncryptor: DynamoDbItemEncryptor.DynamoDbItemEncryptorClient
-    // TODO scan beacon config
+    // TODO beacon config
   )
 
   predicate ValidTableConfig?(config: TableConfig) {
@@ -28,26 +39,106 @@ module AwsCryptographyDynamoDbEncryptionMiddlewareInternalOperations refines Abs
     tableEncryptionConfigs: map<string, ValidTableConfig>
     // TODO allowed passthrough tables
   )
+
   predicate ValidInternalConfig?(config: InternalConfig)
   {
-    forall tableName <- config.tableEncryptionConfigs
-    ::
-      config.tableEncryptionConfigs[tableName].itemEncryptor.config.tableName == tableName
+    && (forall tableName <- config.tableEncryptionConfigs ::
+        config.tableEncryptionConfigs[tableName].itemEncryptor.config.tableName == tableName)
+    && (forall t :: t in config.tableEncryptionConfigs.Keys ==>
+        config.tableEncryptionConfigs[t].itemEncryptor.ValidState())
+  }
+
+  function ModifiesInternalConfig(config: InternalConfig) : set<object>
+  {
+    set t <- config.tableEncryptionConfigs.Keys, o <- config.tableEncryptionConfigs[t].itemEncryptor.Modifies :: o
   }
 
   type InternalConfig = Config
 
-  // TODO Not sure why the verifier is not complaining that I am not modeling the itemEncryptor.Modifies...
-  function ModifiesInternalConfig(config: InternalConfig) : set<object>
-  {{}}
+  function method MapError<T>(r : Result<T, EncTypes.Error>) : Result<T, Error> {
+    r.MapFailure(e => AwsCryptographyDynamoDbItemEncryptor(e))
+  }
+
+  function method MakeError<X>(s : string) : Result<X, Error>
+  {
+    Failure(Error.DynamoDbEncryptionMiddlewareInternalException(message := s))
+  }
+
+  predicate SameOption<X>(x : Option<X>, y : Option<X>)
+  {
+    (x.Some? && y.Some?) || (x.None? && y.None?)
+  }
 
   predicate PutItemInputTransformEnsuresPublicly(input: PutItemInputTransformInput, output: Result<PutItemInputTransformOutput, Error>)
   {true}
 
   method PutItemInputTransform(config: InternalConfig, input: PutItemInputTransformInput)
     returns (output: Result<PutItemInputTransformOutput, Error>)
+
+    //= specification/dynamodb-encryption-client/ddb-sdk-integration.md#encrypt-before-putitem
+    //= type=implication
+    //# If there exists an Item Encryptor specified within the
+    //# [DynamoDB Encryption Client Config](#dynamodb-encryption-client-configuration)
+    //# with a [DynamoDB Table Name](./ddb-item-encryptor.md#dynamodb-table-name)
+    //# equal to `TableName` in the request,
+    //# this PutItem request MUST NOT contain a `ConditionExpression`.
+
+    //= specification/dynamodb-encryption-client/ddb-sdk-integration.md#encrypt-before-putitem
+    //= type=implication
+    //# If the above validation fails,
+    //# the client MUST NOT make a network call to DynamoDB,
+    //# and PutItem MUST yield an error.
+    ensures
+      && input.sdkInput.TableName in config.tableEncryptionConfigs
+      && (input.sdkInput.ConditionExpression.Some? || input.sdkInput.ConditionalOperator.Some?)
+      ==> output.Failure?
+
+    ensures output.Success? && input.sdkInput.TableName !in config.tableEncryptionConfigs ==>
+            output.value.transformedInput == input.sdkInput
+
+    //= specification/dynamodb-encryption-client/ddb-sdk-integration.md#encrypt-before-putitem
+    //= type=implication
+    //# If the request is validated,
+    //# it MUST be modified before a network call is made to DynamoDB
+    //# if there exists an Item Encryptor specified within the
+    //# [DynamoDB Encryption Client Config](#dynamodb-encryption-client-configuration)
+    //# with a [DynamoDB Table Name](./ddb-item-encryptor.md#dynamodb-table-name)
+    //# equal to `TableName` in the request.
+    ensures output.Success? && input.sdkInput.TableName in config.tableEncryptionConfigs ==>
+      && (|config.tableEncryptionConfigs[input.sdkInput.TableName].itemEncryptor.History.EncryptItem| ==
+          |old(config.tableEncryptionConfigs[input.sdkInput.TableName].itemEncryptor.History.EncryptItem)|+1)
+      && (Seq.Last(config.tableEncryptionConfigs[input.sdkInput.TableName].itemEncryptor.History.EncryptItem).output.Success?)
+
+      //= specification/dynamodb-encryption-client/ddb-sdk-integration.md#encrypt-before-putitem
+      //= type=implication
+      //# This [Item Encryptor](./ddb-item-encryptor.md) MUST perform
+      //# [Encrypt Item](./encrypt-item.md),
+      //# where the input [DynamoDB Item](./encrypt-item.md#dynamodb-item)
+      //# is the `Item` field in the original request.
+      && Seq.Last(config.tableEncryptionConfigs[input.sdkInput.TableName].itemEncryptor.History.EncryptItem).input.plaintextItem
+        == input.sdkInput.Item
+
+      //= specification/dynamodb-encryption-client/ddb-sdk-integration.md#encrypt-before-putitem
+      //= type=implication
+      //# The PutItem request's `Item` field MUST be replaced
+      //# with a value that is equivalent to
+      //# the result [Encrypted DynamoDB Item](./encrypt-item.md#encrypted-dynamodb-item)
+      //# calculated above.
+      && (Seq.Last(config.tableEncryptionConfigs[input.sdkInput.TableName].itemEncryptor.History.EncryptItem).output.value.encryptedItem ==
+        output.value.transformedInput.Item)
   {
-      return Failure(DynamoDbEncryptionMiddlewareInternalException(message:="Unimplemented"));
+    if input.sdkInput.TableName !in config.tableEncryptionConfigs {
+      return Success(PutItemInputTransformOutput(transformedInput := input.sdkInput));
+    }
+    if input.sdkInput.ConditionExpression.Some? || input.sdkInput.ConditionalOperator.Some? {
+      return MakeError("Condition Expressions not supported in PutItem with Encryption.");
+    }
+    var tableConfig := config.tableEncryptionConfigs[input.sdkInput.TableName];
+    var encryptRes := tableConfig.itemEncryptor.EncryptItem(
+      EncTypes.EncryptItemInput(plaintextItem:=input.sdkInput.Item)
+    );
+    var encrypted :- MapError(encryptRes);
+    return Success(PutItemInputTransformOutput(transformedInput := input.sdkInput.(Item := encrypted.encryptedItem)));
   }
 
   predicate PutItemOutputTransformEnsuresPublicly(input: PutItemOutputTransformInput, output: Result<PutItemOutputTransformOutput, Error>)
@@ -56,7 +147,7 @@ module AwsCryptographyDynamoDbEncryptionMiddlewareInternalOperations refines Abs
   method PutItemOutputTransform(config: InternalConfig, input: PutItemOutputTransformInput)
     returns (output: Result<PutItemOutputTransformOutput, Error>)
   {
-      return Failure(DynamoDbEncryptionMiddlewareInternalException(message:="Unimplemented"));
+    return Success(PutItemOutputTransformOutput(transformedOutput := input.sdkOutput));
   }
 
   predicate GetItemInputTransformEnsuresPublicly(input: GetItemInputTransformInput, output: Result<GetItemInputTransformOutput, Error>)
@@ -65,7 +156,7 @@ module AwsCryptographyDynamoDbEncryptionMiddlewareInternalOperations refines Abs
   method GetItemInputTransform(config: InternalConfig, input: GetItemInputTransformInput)
     returns (output: Result<GetItemInputTransformOutput, Error>)
   {
-      return Failure(DynamoDbEncryptionMiddlewareInternalException(message:="Unimplemented"));
+    return Success(GetItemInputTransformOutput(transformedInput := input.sdkInput));
   }
 
   predicate GetItemOutputTransformEnsuresPublicly(input: GetItemOutputTransformInput, output: Result<GetItemOutputTransformOutput, Error>)
@@ -73,8 +164,51 @@ module AwsCryptographyDynamoDbEncryptionMiddlewareInternalOperations refines Abs
 
   method GetItemOutputTransform(config: InternalConfig, input: GetItemOutputTransformInput)
     returns (output: Result<GetItemOutputTransformOutput, Error>)
+
+    //= specification/dynamodb-encryption-client/ddb-sdk-integration.md#decrypt-after-getitem
+    //= type=implication
+    //# After a [GetItem](https://docs.aws.amazon.com/amazondynamodb/latest/APIReference/API_GetItem.html)
+    //# call is made to DynamoDB,
+    //# the resulting response MUST be modified before
+    //# being returned to the caller if there exists
+    //# an Item Encryptor specified within the [DynamoDB Encryption Client Config](#dynamodb-encryption-client-configuration)
+    //# with a [DynamoDB Table Name](./ddb-item-encryptor.md#dynamodb-table-name)
+    //# equal to the `TableName` on the GetItem request.
+    ensures output.Success? && input.originalInput.TableName !in config.tableEncryptionConfigs ==> output.value.transformedOutput == input.sdkOutput
+    ensures output.Success? && input.sdkOutput.Item.None? ==> output.value.transformedOutput.Item.None?
+    ensures output.Success? && input.originalInput.TableName in config.tableEncryptionConfigs && input.sdkOutput.Item.Some? ==>
+      && (|config.tableEncryptionConfigs[input.originalInput.TableName].itemEncryptor.History.DecryptItem| ==
+          |old(config.tableEncryptionConfigs[input.originalInput.TableName].itemEncryptor.History.DecryptItem)|+1)
+      && (Seq.Last(config.tableEncryptionConfigs[input.originalInput.TableName].itemEncryptor.History.DecryptItem).output.Success?)
+
+      //= specification/dynamodb-encryption-client/ddb-sdk-integration.md#decrypt-after-getitem
+      //= type=implication
+      //# The [Item Encryptor](./ddb-item-encryptor.md) MUST perform
+      //# [Decrypt Item](./decrypt-item.md) where the input
+      //# [DynamoDB Item](./decrypt-item.md#dynamodb-item)
+      //# is the `Item` field in the original response
+      && Seq.Last(config.tableEncryptionConfigs[input.originalInput.TableName].itemEncryptor.History.DecryptItem).input.encryptedItem
+        == input.sdkOutput.Item.value
+
+      //= specification/dynamodb-encryption-client/ddb-sdk-integration.md#decrypt-after-getitem
+      //= type=implication
+      //# The GetItem request's `Item` field MUST be replaced
+      //# with a value that is equivalent to
+      //# the resulting decrypted [DynamoDB Item](./decrypt-item.md#dynamodb-item-1).
+      && output.value.transformedOutput.Item.Some?
+      && (Seq.Last(config.tableEncryptionConfigs[input.originalInput.TableName].itemEncryptor.History.DecryptItem).output.value.plaintextItem ==
+        output.value.transformedOutput.Item.value)
   {
-      return Failure(DynamoDbEncryptionMiddlewareInternalException(message:="Unimplemented"));
+    var tablename := input.originalInput.TableName;
+    if tablename !in config.tableEncryptionConfigs || input.sdkOutput.Item.None? {
+      return Success(GetItemOutputTransformOutput(transformedOutput := input.sdkOutput));
+    }
+    var tableConfig := config.tableEncryptionConfigs[tablename];
+    var decryptRes := tableConfig.itemEncryptor.DecryptItem(
+      EncTypes.DecryptItemInput(encryptedItem:=input.sdkOutput.Item.value)
+    );
+    var decrypted :- MapError(decryptRes);
+    return Success(GetItemOutputTransformOutput(transformedOutput := input.sdkOutput.(Item := Some(decrypted.plaintextItem))));
   }
 
   predicate UpdateItemInputTransformEnsuresPublicly(input: UpdateItemInputTransformInput, output: Result<UpdateItemInputTransformOutput, Error>)
@@ -82,8 +216,32 @@ module AwsCryptographyDynamoDbEncryptionMiddlewareInternalOperations refines Abs
 
   method UpdateItemInputTransform(config: InternalConfig, input: UpdateItemInputTransformInput)
     returns (output: Result<UpdateItemInputTransformOutput, Error>)
+
+    //= specification/dynamodb-encryption-client/ddb-sdk-integration.md#validate-before-updateitem
+    //= type=implication
+    //# Before a [UpdateItem](https://docs.aws.amazon.com/amazondynamodb/latest/APIReference/API_UpdateItem.html)
+    //# call is made to DynamoDB,
+    //# the request MUST fail, and the client make no network call to DynamoDB,
+    //# if there exists an Item Encryptor
+    //# specified within the [DynamoDB Encryption Client Config](#dynamodb-encryption-client-configuration)
+    //# with a [DynamoDB Table Name](./ddb-item-encryptor.md#dynamodb-table-name)
+    //# equal to `TableName` in the request.
+    ensures input.sdkInput.TableName in config.tableEncryptionConfigs ==> output.Failure?
+
+    //= specification/dynamodb-encryption-client/ddb-sdk-integration.md#validate-before-updateitem
+    //= type=implication
+    //# If no such Item Encryptor exists,
+    //# there MUST NOT be any modification
+    //# to the UpdateItem request.
+    ensures input.sdkInput.TableName !in config.tableEncryptionConfigs ==>
+      && output.Success?
+      && output.value.transformedInput == input.sdkInput
   {
+    if input.sdkInput.TableName in config.tableEncryptionConfigs {
       return Failure(DynamoDbEncryptionMiddlewareInternalException(message:="Unimplemented"));
+    } else {
+      return Success(UpdateItemInputTransformOutput(transformedInput := input.sdkInput));
+    }
   }
 
   predicate UpdateItemOutputTransformEnsuresPublicly(input: UpdateItemOutputTransformInput, output: Result<UpdateItemOutputTransformOutput, Error>)
@@ -92,7 +250,7 @@ module AwsCryptographyDynamoDbEncryptionMiddlewareInternalOperations refines Abs
   method UpdateItemOutputTransform(config: InternalConfig, input: UpdateItemOutputTransformInput)
     returns (output: Result<UpdateItemOutputTransformOutput, Error>)
   {
-      return Failure(DynamoDbEncryptionMiddlewareInternalException(message:="Unimplemented"));
+    return Success(UpdateItemOutputTransformOutput(transformedOutput := input.sdkOutput));
   }
 
   predicate BatchWriteItemInputTransformEnsuresPublicly(input: BatchWriteItemInputTransformInput, output: Result<BatchWriteItemInputTransformOutput, Error>)
@@ -100,8 +258,62 @@ module AwsCryptographyDynamoDbEncryptionMiddlewareInternalOperations refines Abs
 
   method BatchWriteItemInputTransform(config: InternalConfig, input: BatchWriteItemInputTransformInput)
     returns (output: Result<BatchWriteItemInputTransformOutput, Error>)
+    ensures output.Success? ==>
+      && (input.sdkInput.RequestItems.Keys == output.value.transformedInput.RequestItems.Keys)
+      && forall k <- input.sdkInput.RequestItems.Keys ::
+        |input.sdkInput.RequestItems[k]| == |output.value.transformedInput.RequestItems[k]|
   {
-      return Failure(DynamoDbEncryptionMiddlewareInternalException(message:="Unimplemented"));
+    var items := input.sdkInput.RequestItems.Keys;
+    var result : map<DDB.TableName, DDB.WriteRequests> := map[];
+    while items != {}
+      decreases |items|
+      invariant items <= input.sdkInput.RequestItems.Keys
+      invariant result.Keys + items == input.sdkInput.RequestItems.Keys
+      invariant forall k <- result.Keys ::
+        |input.sdkInput.RequestItems[k]| == |result[k]|
+
+    {
+      var item :| item in items;
+      items := items - { item };
+      var value : DDB.WriteRequests := input.sdkInput.RequestItems[item];
+      if item in config.tableEncryptionConfigs {
+        var tableConfig := config.tableEncryptionConfigs[item];
+        var decryptedItem : seq<DDB.WriteRequest> := [];
+        for x := 0 to |value|
+          invariant |decryptedItem| == x
+        {
+          var req : DDB.WriteRequest := value[x];
+          if req.PutRequest.None? {
+            decryptedItem := decryptedItem + [req];
+          } else {
+            //= specification/dynamodb-encryption-client/ddb-sdk-integration.md#encrypt-before-batchwriteitem
+            //# For each `PutRequest` under each key in `RequestItems`,
+            //# if there is an Item Encryptor with [DynamoDB Table Name](./ddb-item-encryptor.md#dynamodb-table-name) equal to the key,
+            //# that Item Encryptor MUST perform [Encrypt Item](./encrypt-item.md) where the input
+            //# [DynamoDB Item](./encrypt-item.md#dynamodb-item) is the `Item` field in this `PutRequest`
+            var decryptRes := tableConfig.itemEncryptor.EncryptItem(EncTypes.EncryptItemInput(plaintextItem:=req.PutRequest.value.Item));
+
+            //= specification/dynamodb-encryption-client/ddb-sdk-integration.md#encrypt-before-batchwriteitem
+            //# If any [Encrypt Item](./encrypt-item.md) fails,
+            //# the client MUST NOT make a network call to DynamoDB,
+            //# and BatchWriteItem MUST yield an error.
+            var decrypted :- MapError(decryptRes);
+
+            //= specification/dynamodb-encryption-client/ddb-sdk-integration.md#encrypt-before-batchwriteitem
+            //# The `Item` field in this `PutRequest` MUST be replaced
+            //# with a value that is equivalent to
+            //# the result [Encrypted DynamoDB Item](./encrypt-item.md#encrypted-dynamodb-item).
+            decryptedItem := decryptedItem + [req.(PutRequest := Some(DDB.PutRequest(Item := decrypted.encryptedItem)))];
+          }
+        }
+        assert |decryptedItem| == |input.sdkInput.RequestItems[item]|;
+        result := result[item := decryptedItem];
+      } else {
+        result := result[item := value];
+      }
+    }
+
+    return Success(BatchWriteItemInputTransformOutput(transformedInput := input.sdkInput.(RequestItems := result)));
   }
 
   predicate BatchWriteItemOutputTransformEnsuresPublicly(input: BatchWriteItemOutputTransformInput, output: Result<BatchWriteItemOutputTransformOutput, Error>)
@@ -110,16 +322,131 @@ module AwsCryptographyDynamoDbEncryptionMiddlewareInternalOperations refines Abs
   method BatchWriteItemOutputTransform(config: InternalConfig, input: BatchWriteItemOutputTransformInput)
     returns (output: Result<BatchWriteItemOutputTransformOutput, Error>)
   {
-      return Failure(DynamoDbEncryptionMiddlewareInternalException(message:="Unimplemented"));
+    return Success(BatchWriteItemOutputTransformOutput(transformedOutput := input.sdkOutput));
   }
 
   predicate TransactWriteItemsInputTransformEnsuresPublicly(input: TransactWriteItemsInputTransformInput, output: Result<TransactWriteItemsInputTransformOutput, Error>)
   {true}
 
+  function ExpectedEncryptCount(max : nat, table : string, config: InternalConfig, input: TransactWriteItemsInputTransformInput) : nat
+    requires max <= |input.sdkInput.TransactItems|
+  {
+    |set x <- input.sdkInput.TransactItems[0..max] ::
+      (x.Put.Some? && x.Put.value.TableName in config.tableEncryptionConfigs && x.Put.value.TableName == table)|
+  }
+
   method TransactWriteItemsInputTransform(config: InternalConfig, input: TransactWriteItemsInputTransformInput)
     returns (output: Result<TransactWriteItemsInputTransformOutput, Error>)
+
+    ensures output.Success? ==> |output.value.transformedInput.TransactItems| == |input.sdkInput.TransactItems|
+
+    //= specification/dynamodb-encryption-client/ddb-sdk-integration.md#encrypt-before-transactwriteitems
+    //= type=implication
+    //# - The client MUST fail if in the `ConditionCheck` field has a `TableName` which matches
+    //# the [DynamoDB Table Name](./ddb-item-encryptor.md#dynamodb-table-name)
+    //# of any Item Encryptor specified within the
+    //# [DynamoDB Encryption Client Config](#dynamodb-encryption-client-configuration)
+    ensures output.Success? ==>
+      forall item <- input.sdkInput.TransactItems ::
+        (item.ConditionCheck.None? || item.ConditionCheck.value.TableName !in config.tableEncryptionConfigs)
+
+    //= specification/dynamodb-encryption-client/ddb-sdk-integration.md#encrypt-before-transactwriteitems
+    //= type=implication
+    //# - The client MUST fail if in the `Delete` field has a `TableName` which matches
+    //# the [DynamoDB Table Name](./ddb-item-encryptor.md#dynamodb-table-name)
+    //# of any Item Encryptor specified within the
+    //# [DynamoDB Encryption Client Config](#dynamodb-encryption-client-configuration)
+    //# and also has a `ConditionExpression`
+    ensures output.Success? ==>
+      forall item <- input.sdkInput.TransactItems ::
+        || item.Delete.None?
+        || item.Delete.value.TableName !in config.tableEncryptionConfigs
+        || item.Delete.value.ConditionExpression.None?
+
+    //= specification/dynamodb-encryption-client/ddb-sdk-integration.md#encrypt-before-transactwriteitems
+    //= type=implication
+    //# - The client MUST fail if in the `Update` field has a `TableName` which matches
+    //# the [DynamoDB Table Name](./ddb-item-encryptor.md#dynamodb-table-name)
+    //# of any Item Encryptor specified within the
+    //# [DynamoDB Encryption Client Config](#dynamodb-encryption-client-configuration)
+    ensures output.Success? ==>
+      forall item <- input.sdkInput.TransactItems ::
+        (item.Update.None? || item.Update.value.TableName !in config.tableEncryptionConfigs)
+
+    //= specification/dynamodb-encryption-client/ddb-sdk-integration.md#encrypt-before-transactwriteitems
+    //= type=implication
+    //# - The client MUST fail if in the `Put` field has a `TableName` which matches
+    //# the [DynamoDB Table Name](./ddb-item-encryptor.md#dynamodb-table-name)
+    //# of any Item Encryptor specified within the
+    //# [DynamoDB Encryption Client Config](#dynamodb-encryption-client-configuration)
+    //# and also has a `ConditionExpression`
+    ensures output.Success? ==>
+      forall item <- input.sdkInput.TransactItems ::
+        || item.Put.None?
+        || item.Put.value.TableName !in config.tableEncryptionConfigs
+        || item.Put.value.ConditionExpression.None?
+
   {
-      return Failure(DynamoDbEncryptionMiddlewareInternalException(message:="Unimplemented"));
+    var result : seq<DDB.TransactWriteItem> := [];
+    for x := 0 to |input.sdkInput.TransactItems|
+      invariant |result| == x
+      invariant forall i : nat | 0 <= i < |result| ::
+        var item := input.sdkInput.TransactItems[i];
+        && (|| item.ConditionCheck.None?
+            || item.ConditionCheck.value.TableName !in config.tableEncryptionConfigs)
+        && (|| item.Delete.None?
+            || item.Delete.value.TableName !in config.tableEncryptionConfigs
+            || item.Delete.value.ConditionExpression.None?)
+        && (|| item.Update.None?
+            || item.Update.value.TableName !in config.tableEncryptionConfigs)
+        && (|| item.Put.None?
+            || item.Put.value.TableName !in config.tableEncryptionConfigs
+            || item.Put.value.ConditionExpression.None?)
+    {
+      var item := input.sdkInput.TransactItems[x];
+
+      if item.ConditionCheck.Some? && item.ConditionCheck.value.TableName in config.tableEncryptionConfigs {
+        return MakeError("Condition checks not allowed on encrypted tables (TransactWriteItems ConditionCheck)");
+      }
+      if item.Delete.Some? && item.Delete.value.TableName in config.tableEncryptionConfigs && item.Delete.value.ConditionExpression.Some? {
+        return MakeError("Condition checks not allowed on encrypted tables (TransactWriteItems Delete)");
+      }
+      if item.Update.Some? && item.Update.value.TableName in config.tableEncryptionConfigs {
+          return MakeError("Updates not allowed on encrypted tables (TransactWriteItems Update)");
+      }
+      if item.Put.Some? && item.Put.value.TableName in config.tableEncryptionConfigs {
+        if item.Put.value.ConditionExpression.Some? {
+          return MakeError("Condition checks not allowed on encrypted tables (TransactWriteItems Put)");
+        }
+        var tableConfig := config.tableEncryptionConfigs[item.Put.value.TableName];
+
+        //= specification/dynamodb-encryption-client/ddb-sdk-integration.md#encrypt-before-transactwriteitems
+        //# If the request is valid, for each `Put` in `TransactItems` in the request,
+        //# if a corresponding Item Encryptor exists,
+        //# it MUST perform [Encrypt Item](./encrypt-item.md) where the input
+        //# [DynamoDB Item](./encrypt-item.md#dynamodb-item) is
+        //# the `Item` field in this `Put`
+        var encryptRes := tableConfig.itemEncryptor.EncryptItem(
+          EncTypes.EncryptItemInput(plaintextItem:=item.Put.value.Item)
+        );
+
+        //= specification/dynamodb-encryption-client/ddb-sdk-integration.md#encrypt-before-transactwriteitems
+        //# If any of the above validation fails, or any [Encrypt Item](./encrypt-item.md) fails,
+        //# the client MUST NOT make a network call to DynamoDB and
+        //# TransactWriteItems MUST yield an error.
+        var encrypted :- MapError(encryptRes);
+
+        //= specification/dynamodb-encryption-client/ddb-sdk-integration.md#encrypt-before-transactwriteitems
+        //# The `Item` field in this `Put` MUST be replaced
+        //# with a value that is equivalent to
+        //# the resulting [Encrypted DynamoDB Item](./encrypt-item.md#encrypted-dynamodb-item).
+        var put := Some(item.Put.value.(Item := encrypted.encryptedItem));
+        result := result + [item.(Put := put)];
+      } else {
+        result := result + [item];
+      }
+    }
+    return Success(TransactWriteItemsInputTransformOutput(transformedInput := input.sdkInput.(TransactItems := result)));
   }
 
   predicate TransactWriteItemsOutputTransformEnsuresPublicly(input: TransactWriteItemsOutputTransformInput, output: Result<TransactWriteItemsOutputTransformOutput, Error>)
@@ -128,7 +455,7 @@ module AwsCryptographyDynamoDbEncryptionMiddlewareInternalOperations refines Abs
   method TransactWriteItemsOutputTransform(config: InternalConfig, input: TransactWriteItemsOutputTransformInput)
     returns (output: Result<TransactWriteItemsOutputTransformOutput, Error>)
   {
-      return Failure(DynamoDbEncryptionMiddlewareInternalException(message:="Unimplemented"));
+    return Success(TransactWriteItemsOutputTransformOutput(transformedOutput := input.sdkOutput));
   }
 
   predicate BatchGetItemInputTransformEnsuresPublicly(input: BatchGetItemInputTransformInput, output: Result<BatchGetItemInputTransformOutput, Error>)
@@ -137,7 +464,7 @@ module AwsCryptographyDynamoDbEncryptionMiddlewareInternalOperations refines Abs
   method BatchGetItemInputTransform(config: InternalConfig, input: BatchGetItemInputTransformInput)
     returns (output: Result<BatchGetItemInputTransformOutput, Error>)
   {
-      return Failure(DynamoDbEncryptionMiddlewareInternalException(message:="Unimplemented"));
+    return Success(BatchGetItemInputTransformOutput(transformedInput := input.sdkInput));
   }
 
   predicate BatchGetItemOutputTransformEnsuresPublicly(input: BatchGetItemOutputTransformInput, output: Result<BatchGetItemOutputTransformOutput, Error>)
@@ -145,8 +472,53 @@ module AwsCryptographyDynamoDbEncryptionMiddlewareInternalOperations refines Abs
 
   method BatchGetItemOutputTransform(config: InternalConfig, input: BatchGetItemOutputTransformInput)
     returns (output: Result<BatchGetItemOutputTransformOutput, Error>)
+    ensures output.Success? ==> SameOption(input.sdkOutput.Responses, output.value.transformedOutput.Responses)
+    ensures output.Success? && input.sdkOutput.Responses.Some? ==>
+      && output.value.transformedOutput.Responses.Some?
+      && input.sdkOutput.Responses.value.Keys == output.value.transformedOutput.Responses.value.Keys
   {
-      return Failure(DynamoDbEncryptionMiddlewareInternalException(message:="Unimplemented"));
+    if input.sdkOutput.Responses.None? {
+      return Success(BatchGetItemOutputTransformOutput(transformedOutput := input.sdkOutput));
+    }
+    var items := input.sdkOutput.Responses.value.Keys;
+    var result := map[];
+    while items != {}
+      decreases |items|
+      invariant items <= input.sdkOutput.Responses.value.Keys
+      invariant result.Keys + items == input.sdkOutput.Responses.value.Keys
+    {
+      var item :| item in items;
+      items := items - { item };
+      var value := input.sdkOutput.Responses.value[item];
+      if item in config.tableEncryptionConfigs {
+        var tableConfig := config.tableEncryptionConfigs[item];
+        var decryptedItem : DDB.ItemList := [];
+        for x := 0 to |value| {
+          //= specification/dynamodb-encryption-client/ddb-sdk-integration.md#decrypt-after-batchgetitem
+          //# For each list item under each key in `Responses`,
+          //# if there is a configured Item Encryptor with  [DynamoDB Table Name](./ddb-item-encryptor.md#dynamodb-table-name) equal to the key,
+          //# that Item Encryptor MUST perform [Decrypt Item](./decrypt-item.md) where the input
+          //# [DynamoDB Item](./decrypt-item.md#dynamodb-item)
+          //# is the `Item` field in the original response.
+          var decryptRes := tableConfig.itemEncryptor.DecryptItem(EncTypes.DecryptItemInput(encryptedItem:=value[x]));
+
+          //= specification/dynamodb-encryption-client/ddb-sdk-integration.md#decrypt-after-batchgetitem
+          //# If any [Decrypt Item](./decrypt-item.md) operation fails,
+          //# BatchGetItem MUST yield an error.
+          var decrypted :- MapError(decryptRes);
+
+          //= specification/dynamodb-encryption-client/ddb-sdk-integration.md#decrypt-after-batchgetitem
+          //# Each of these items on the original repsonse MUST be replaced
+          //# with a value that is equivalent to
+          //# the resulting decrypted [DynamoDB Item](./decrypt-item.md#dynamodb-item-1).
+          decryptedItem := decryptedItem + [decrypted.plaintextItem];
+        }
+        result := result + map[item := decryptedItem];
+      } else {
+        result := result + map[item := value];
+      }
+    }
+    return Success(BatchGetItemOutputTransformOutput(transformedOutput := input.sdkOutput.(Responses := Some(result))));
   }
 
   predicate ScanInputTransformEnsuresPublicly(input: ScanInputTransformInput, output: Result<ScanInputTransformOutput, Error>)
@@ -155,7 +527,7 @@ module AwsCryptographyDynamoDbEncryptionMiddlewareInternalOperations refines Abs
   method ScanInputTransform(config: InternalConfig, input: ScanInputTransformInput)
     returns (output: Result<ScanInputTransformOutput, Error>)
   {
-      return Failure(DynamoDbEncryptionMiddlewareInternalException(message:="Unimplemented"));
+    return Success(ScanInputTransformOutput(transformedInput := input.sdkInput));
   }
 
   predicate ScanOutputTransformEnsuresPublicly(input: ScanOutputTransformInput, output: Result<ScanOutputTransformOutput, Error>)
@@ -163,8 +535,79 @@ module AwsCryptographyDynamoDbEncryptionMiddlewareInternalOperations refines Abs
 
   method ScanOutputTransform(config: InternalConfig, input: ScanOutputTransformInput)
     returns (output: Result<ScanOutputTransformOutput, Error>)
+
+    ensures input.originalInput.TableName !in config.tableEncryptionConfigs || input.sdkOutput.ItemList.None? ==>
+      && output.Success?
+      && output.value.transformedOutput == input.sdkOutput
+
+    ensures output.Success?  && input.sdkOutput.ItemList.None?  ==> output.value.transformedOutput.ItemList.None?
+    ensures output.Success?  && input.sdkOutput.ItemList.Some?  ==>
+      && output.value.transformedOutput.ItemList.Some?
+      && |output.value.transformedOutput.ItemList.value| == |input.sdkOutput.ItemList.value|
+
+    ensures output.Success? && input.sdkOutput.ItemList.Some? && input.originalInput.TableName in config.tableEncryptionConfigs ==>
+      && (|config.tableEncryptionConfigs[input.originalInput.TableName].itemEncryptor.History.DecryptItem| ==
+          |old(config.tableEncryptionConfigs[input.originalInput.TableName].itemEncryptor.History.DecryptItem)| + |input.sdkOutput.ItemList.value|)
+
+      && (forall i : nat | |old(config.tableEncryptionConfigs[input.originalInput.TableName].itemEncryptor.History.DecryptItem)|
+          <= i <
+          |input.sdkOutput.ItemList.value| + |old(config.tableEncryptionConfigs[input.originalInput.TableName].itemEncryptor.History.DecryptItem)| ::
+          (
+            //= specification/dynamodb-encryption-client/ddb-sdk-integration.md#decrypt-after-scan
+            //= type=implication
+            //# If any [Decrypt Item](./decrypt-item.md) operation fails,
+            //# the client MUST NOT make a network call to DynamoDB
+            //# and Scan MUST yield an error.
+            && config.tableEncryptionConfigs[input.originalInput.TableName].itemEncryptor.History.DecryptItem[i].output.Success?
+
+            //= specification/dynamodb-encryption-client/ddb-sdk-integration.md#decrypt-after-scan
+            //= type=implication
+            //# For each list entry in `Items` in the response,
+            //# if there exists an Item Encryptor specified within the
+            //# [DynamoDB Encryption Client Config](#dynamodb-encryption-client-configuration)
+            //# with a [DynamoDB Table Name](./ddb-item-encryptor.md#dynamodb-table-name)
+            //# equal to the `TableName` on the request,
+            //# the corresponding Item Encryptor MUST perform [Decrypt Item](./decrypt-item.md)
+            //# where the input [DynamoDB Item](./decrypt-item.md#dynamodb-item)
+            //# is this list entry.
+            && config.tableEncryptionConfigs[input.originalInput.TableName].itemEncryptor.History.DecryptItem[i].input.encryptedItem ==
+              input.sdkOutput.ItemList.value[i-|old(config.tableEncryptionConfigs[input.originalInput.TableName].itemEncryptor.History.DecryptItem)|]
+
+            //= specification/dynamodb-encryption-client/ddb-sdk-integration.md#decrypt-after-scan
+            //= type=implication
+            //# Each of these entries on the original repsonse MUST be replaced
+            //# with the resulting decrypted
+            //# [DynamoDB Item](./decrypt-item.md#dynamodb-item-1).
+            && config.tableEncryptionConfigs[input.originalInput.TableName].itemEncryptor.History.DecryptItem[i].output.value.plaintextItem ==
+               output.value.transformedOutput.ItemList.value[i-|old(config.tableEncryptionConfigs[input.originalInput.TableName].itemEncryptor.History.DecryptItem)|]
+          )
+         )
   {
-      return Failure(DynamoDbEncryptionMiddlewareInternalException(message:="Unimplemented"));
+    var tableName := input.originalInput.TableName;
+    if tableName !in config.tableEncryptionConfigs || input.sdkOutput.ItemList.None? {
+      return Success(ScanOutputTransformOutput(transformedOutput := input.sdkOutput));
+    }
+    var tableConfig := config.tableEncryptionConfigs[tableName];
+    var decryptedItem : DDB.ItemList := [];
+    var list := input.sdkOutput.ItemList.value;
+    ghost var historySize := |tableConfig.itemEncryptor.History.DecryptItem|;
+    for x := 0 to |list|
+      invariant |decryptedItem| == x
+      invariant
+        && (|tableConfig.itemEncryptor.History.DecryptItem| ==
+            |old(tableConfig.itemEncryptor.History.DecryptItem)| + |decryptedItem|)
+
+      invariant (forall i : nat | historySize <= i < |decryptedItem|+historySize ::
+        var item := tableConfig.itemEncryptor.History.DecryptItem[i];
+        && item.output.Success?
+        && item.input.encryptedItem == input.sdkOutput.ItemList.value[i-historySize]
+        && item.output.value.plaintextItem == decryptedItem[i-historySize])
+    {
+      var decryptRes := tableConfig.itemEncryptor.DecryptItem(EncTypes.DecryptItemInput(encryptedItem:=list[x]));
+      var decrypted :- MapError(decryptRes);
+      decryptedItem := decryptedItem + [decrypted.plaintextItem];
+    }
+    return Success(ScanOutputTransformOutput(transformedOutput := input.sdkOutput.(ItemList := Some(decryptedItem))));
   }
 
   predicate QueryInputTransformEnsuresPublicly(input: QueryInputTransformInput, output: Result<QueryInputTransformOutput, Error>)
@@ -173,7 +616,7 @@ module AwsCryptographyDynamoDbEncryptionMiddlewareInternalOperations refines Abs
   method QueryInputTransform(config: InternalConfig, input: QueryInputTransformInput)
     returns (output: Result<QueryInputTransformOutput, Error>)
   {
-      return Failure(DynamoDbEncryptionMiddlewareInternalException(message:="Unimplemented"));
+    return Success(QueryInputTransformOutput(transformedInput := input.sdkInput));
   }
 
   predicate QueryOutputTransformEnsuresPublicly(input: QueryOutputTransformInput, output: Result<QueryOutputTransformOutput, Error>)
@@ -181,8 +624,99 @@ module AwsCryptographyDynamoDbEncryptionMiddlewareInternalOperations refines Abs
 
   method QueryOutputTransform(config: InternalConfig, input: QueryOutputTransformInput)
     returns (output: Result<QueryOutputTransformOutput, Error>)
+
+    ensures input.originalInput.TableName !in config.tableEncryptionConfigs || input.sdkOutput.ItemList.None? ==>
+      && output.Success?
+      && output.value.transformedOutput == input.sdkOutput
+
+    ensures output.Success?  && input.sdkOutput.ItemList.Some?  ==>
+      && output.value.transformedOutput.ItemList.Some?
+      && |output.value.transformedOutput.ItemList.value| == |input.sdkOutput.ItemList.value|
+
+    ensures output.Success?  && input.sdkOutput.ItemList.None?  ==>
+      && output.value.transformedOutput.ItemList.None?
+
+    ensures output.Success? && input.sdkOutput.ItemList.Some? && input.originalInput.TableName in config.tableEncryptionConfigs ==>
+      && (|config.tableEncryptionConfigs[input.originalInput.TableName].itemEncryptor.History.DecryptItem| ==
+          |old(config.tableEncryptionConfigs[input.originalInput.TableName].itemEncryptor.History.DecryptItem)| + |input.sdkOutput.ItemList.value|)
+
+      && (forall i : nat | |old(config.tableEncryptionConfigs[input.originalInput.TableName].itemEncryptor.History.DecryptItem)|
+          <= i <
+          |input.sdkOutput.ItemList.value| + |old(config.tableEncryptionConfigs[input.originalInput.TableName].itemEncryptor.History.DecryptItem)| ::
+          (
+            //= specification/dynamodb-encryption-client/ddb-sdk-integration.md#decrypt-after-query
+            //= type=implication
+            //# If any [Decrypt Item](./decrypt-item.md) fails,
+            //# the client MUST NOT make a network call to DynamoDB
+            //# and Query MUST yield an error.
+            && config.tableEncryptionConfigs[input.originalInput.TableName].itemEncryptor.History.DecryptItem[i].output.Success?
+
+            //= specification/dynamodb-encryption-client/ddb-sdk-integration.md#decrypt-after-query
+            //= type=implication
+            //# For each list entry in `Items` in the response,
+            //# if there exists an Item Encryptor specified within the
+            //# [DynamoDB Encryption Client Config](#dynamodb-encryption-client-configuration)
+            //# with a [DynamoDB Table Name](./ddb-item-encryptor.md#dynamodb-table-name)
+            //# equal to the `TableName` on the request,
+            //# the corresponding Item Encryptor MUST perform [Decrypt Item](./decrypt-item.md)
+            //# where the input [DynamoDB Item](./decrypt-item.md#dynamodb-item)
+            //# is this list entry.
+            && config.tableEncryptionConfigs[input.originalInput.TableName].itemEncryptor.History.DecryptItem[i].input.encryptedItem ==
+              input.sdkOutput.ItemList.value[i-|old(config.tableEncryptionConfigs[input.originalInput.TableName].itemEncryptor.History.DecryptItem)|]
+
+            //= specification/dynamodb-encryption-client/ddb-sdk-integration.md#decrypt-after-query
+            //= type=implication
+            //# Each of these entries on the original repsonse MUST be replaced
+            //# with the resulting decrypted [DynamoDB Item](./decrypt-item.md#dynamodb-item-1).
+            && config.tableEncryptionConfigs[input.originalInput.TableName].itemEncryptor.History.DecryptItem[i].output.value.plaintextItem ==
+               output.value.transformedOutput.ItemList.value[i-|old(config.tableEncryptionConfigs[input.originalInput.TableName].itemEncryptor.History.DecryptItem)|]
+          )
+         )
   {
-      return Failure(DynamoDbEncryptionMiddlewareInternalException(message:="Unimplemented"));
+    var tableName := input.originalInput.TableName;
+    if tableName !in config.tableEncryptionConfigs || input.sdkOutput.ItemList.None? {
+      return Success(QueryOutputTransformOutput(transformedOutput := input.sdkOutput));
+    }
+    var tableConfig := config.tableEncryptionConfigs[tableName];
+    var decryptedItem : DDB.ItemList := [];
+    var list := input.sdkOutput.ItemList.value;
+    ghost var historySize := |tableConfig.itemEncryptor.History.DecryptItem|;
+    for x := 0 to |list|
+      invariant |decryptedItem| == x
+
+      invariant
+        && (|tableConfig.itemEncryptor.History.DecryptItem| ==
+            |old(tableConfig.itemEncryptor.History.DecryptItem)| + |decryptedItem|)
+
+      invariant (forall i : nat | historySize <= i < |decryptedItem|+historySize ::
+        var item := tableConfig.itemEncryptor.History.DecryptItem[i];
+        && item.output.Success?
+        && item.input.encryptedItem == input.sdkOutput.ItemList.value[i-historySize]
+        && item.output.value.plaintextItem == decryptedItem[i-historySize])
+    {
+      //= specification/dynamodb-encryption-client/ddb-sdk-integration.md#decrypt-after-query
+      //# For each list entry in `Items` in the response,
+      //# if there exists an Item Encryptor specified within the
+      //# [DynamoDB Encryption Client Config](#dynamodb-encryption-client-configuration)
+      //# with a [DynamoDB Table Name](./ddb-item-encryptor.md#dynamodb-table-name)
+      //# equal to the `TableName` on the request,
+      //# the corresponding Item Encryptor MUST perform [Decrypt Item](./decrypt-item.md)
+      //# where the input [DynamoDB Item](./decrypt-item.md#dynamodb-item)
+      //# is this list entry.
+      var decryptRes := tableConfig.itemEncryptor.DecryptItem(EncTypes.DecryptItemInput(encryptedItem:=list[x]));
+
+      //= specification/dynamodb-encryption-client/ddb-sdk-integration.md#decrypt-after-query
+      //# If any [Decrypt Item](./decrypt-item.md) fails,
+      //# the client MUST NOT make a network call to DynamoDB
+      //# and Query MUST yield an error.
+      var decrypted :- MapError(decryptRes);
+
+      //= specification/dynamodb-encryption-client/ddb-sdk-integration.md#decrypt-after-query
+      //# Each of these entries on the original repsonse MUST be replaced
+      //# with the resulting decrypted [DynamoDB Item](./decrypt-item.md#dynamodb-item-1).
+      decryptedItem := decryptedItem + [decrypted.plaintextItem];
+    }
+    return Success(QueryOutputTransformOutput(transformedOutput := input.sdkOutput.(ItemList := Some(decryptedItem))));
   }
 
   predicate TransactGetItemsInputTransformEnsuresPublicly(input: TransactGetItemsInputTransformInput, output: Result<TransactGetItemsInputTransformOutput, Error>)
@@ -191,7 +725,7 @@ module AwsCryptographyDynamoDbEncryptionMiddlewareInternalOperations refines Abs
   method TransactGetItemsInputTransform(config: InternalConfig, input: TransactGetItemsInputTransformInput)
     returns (output: Result<TransactGetItemsInputTransformOutput, Error>)
   {
-      return Failure(DynamoDbEncryptionMiddlewareInternalException(message:="Unimplemented"));
+    return Success(TransactGetItemsInputTransformOutput(transformedInput := input.sdkInput));
   }
 
   predicate TransactGetItemsOutputTransformEnsuresPublicly(input: TransactGetItemsOutputTransformInput, output: Result<TransactGetItemsOutputTransformOutput, Error>)
@@ -199,8 +733,60 @@ module AwsCryptographyDynamoDbEncryptionMiddlewareInternalOperations refines Abs
 
   method TransactGetItemsOutputTransform(config: InternalConfig, input: TransactGetItemsOutputTransformInput)
     returns (output: Result<TransactGetItemsOutputTransformOutput, Error>)
+
+    ensures input.sdkOutput.Responses.None? ==>
+      && output.Success?
+      && output.value.transformedOutput == input.sdkOutput
+
+    ensures output.Success? && input.sdkOutput.Responses.Some? ==>
+      && output.value.transformedOutput.Responses.Some?
+      && |output.value.transformedOutput.Responses.value| == |input.originalInput.TransactItems|
   {
-      return Failure(DynamoDbEncryptionMiddlewareInternalException(message:="Unimplemented"));
+    if input.sdkOutput.Responses.None? {
+      return Success(TransactGetItemsOutputTransformOutput(transformedOutput := input.sdkOutput));
+    }
+    if |input.sdkOutput.Responses.value| != |input.originalInput.TransactItems| {
+      return Failure(DynamoDbEncryptionMiddlewareInternalException(message:="Corrupt Original Input for TransactGetItems"));
+    }
+    var decryptedItem : seq<DDB.ItemResponse> := [];
+    var list := input.sdkOutput.Responses.value;
+    for x := 0 to |list|
+      invariant |decryptedItem| == x
+    {
+      var tableName := input.originalInput.TransactItems[x].Get.TableName;
+      if tableName !in config.tableEncryptionConfigs {
+        decryptedItem := decryptedItem + [list[x]];
+      } else {
+        var tableConfig := config.tableEncryptionConfigs[tableName];
+        if list[x].Item.None? {
+          decryptedItem := decryptedItem + [DDB.ItemResponse(Item := None)];
+        } else {
+          //= specification/dynamodb-encryption-client/ddb-sdk-integration.md#decrypt-after-transactgetitems
+          //# For each list item under each key in `Responses`,
+          //# if there exists an Item Encryptor specified within
+          //# the [DynamoDB Encryption Client Config](#dynamodb-encryption-client-configuration)
+          //# with a [DynamoDB Table Name](./ddb-item-encryptor.md#dynamodb-table-name)
+          //# equal to the key,
+          //# the Item Encryptor that corresponds to the key in the request
+          //# MUST perform [Decrypt Item](./decrypt-item.md) where the input
+          //# [DynamoDB Item](./decrypt-item.md#dynamodb-item) is the `Item` in the original response
+          var decryptRes := tableConfig.itemEncryptor.DecryptItem(EncTypes.DecryptItemInput(encryptedItem:=list[x].Item.value));
+
+          //= specification/dynamodb-encryption-client/ddb-sdk-integration.md#decrypt-after-transactgetitems
+          //# If any [Decrypt Item](./decrypt-item.md) fails,
+          //# the client MUST NOT make a network call to DynamoDB
+          //# and TransactGetItems MUST yield an error.
+          var decrypted :- MapError(decryptRes);
+
+          //= specification/dynamodb-encryption-client/ddb-sdk-integration.md#decrypt-after-transactgetitems
+          //# Each of these items on the original repsonse MUST be replaced
+          //# with a value that is equivalent to
+          //# the result [DynamoDB Item](./decrypt-item.md#dynamodb-item-1).
+          decryptedItem := decryptedItem + [DDB.ItemResponse(Item := Some(decrypted.plaintextItem))];
+        }
+      }
+    }
+    return Success(TransactGetItemsOutputTransformOutput(transformedOutput := input.sdkOutput.(Responses := Some(decryptedItem))));
   }
 
   predicate DeleteItemInputTransformEnsuresPublicly(input: DeleteItemInputTransformInput, output: Result<DeleteItemInputTransformOutput, Error>)
@@ -208,8 +794,41 @@ module AwsCryptographyDynamoDbEncryptionMiddlewareInternalOperations refines Abs
 
   method DeleteItemInputTransform(config: InternalConfig, input: DeleteItemInputTransformInput)
     returns (output: Result<DeleteItemInputTransformOutput, Error>)
+
+    //= specification/dynamodb-encryption-client/ddb-sdk-integration.md#validate-before-deleteitem
+      //= type=implication
+      //# Before a [DeleteItem](https://docs.aws.amazon.com/amazondynamodb/latest/APIReference/API_DeleteItem.html)
+      //# call is made to DynamoDB,
+      //# the request MUST fail, and the client make no network call to DynamoDB,
+      //# if the request specifies a `ConditionExpression`,
+      //# and there exists an Item Encryptor specified
+      //# within the [DynamoDB Encryption Client Config](#dynamodb-encryption-client-configuration)
+      //# with a [DynamoDB Table Name](./ddb-item-encryptor.md#dynamodb-table-name)
+      //# equal to `TableName` in the request.
+      ensures
+        && input.sdkInput.TableName in config.tableEncryptionConfigs
+        && (input.sdkInput.ConditionExpression.Some? || input.sdkInput.ConditionalOperator.Some?)
+        ==> output.Failure?
+
+      //= specification/dynamodb-encryption-client/ddb-sdk-integration.md#validate-before-deleteitem
+      //= type=implication
+      //# Otherwise, there MUST NOT be any modification
+      //# to the UpdateItem request.
+      ensures
+        || input.sdkInput.TableName !in config.tableEncryptionConfigs
+        || (input.sdkInput.ConditionExpression.None? && input.sdkInput.ConditionalOperator.None?)
+        ==>
+        && output.Success?
+        && output.value.transformedInput == input.sdkInput
+
   {
-      return Failure(DynamoDbEncryptionMiddlewareInternalException(message:="Unimplemented"));
+    if input.sdkInput.TableName !in config.tableEncryptionConfigs {
+      return Success(DeleteItemInputTransformOutput(transformedInput := input.sdkInput));
+    }
+    if input.sdkInput.ConditionExpression.Some? || input.sdkInput.ConditionalOperator.Some? {
+      return MakeError("Condition Expressions not supported in DeleteItem with Encryption.");
+    }
+    return Success(DeleteItemInputTransformOutput(transformedInput := input.sdkInput));
   }
 
   predicate DeleteItemOutputTransformEnsuresPublicly(input: DeleteItemOutputTransformInput, output: Result<DeleteItemOutputTransformOutput, Error>)
@@ -218,16 +837,40 @@ module AwsCryptographyDynamoDbEncryptionMiddlewareInternalOperations refines Abs
   method DeleteItemOutputTransform(config: InternalConfig, input: DeleteItemOutputTransformInput)
     returns (output: Result<DeleteItemOutputTransformOutput, Error>)
   {
-      return Failure(DynamoDbEncryptionMiddlewareInternalException(message:="Unimplemented"));
+    return Success(DeleteItemOutputTransformOutput(transformedOutput := input.sdkOutput));
   }
 
-    predicate ExecuteStatementInputTransformEnsuresPublicly(input: ExecuteStatementInputTransformInput, output: Result<ExecuteStatementInputTransformOutput, Error>)
+  predicate ExecuteStatementInputTransformEnsuresPublicly(input: ExecuteStatementInputTransformInput, output: Result<ExecuteStatementInputTransformOutput, Error>)
   {true}
 
   method ExecuteStatementInputTransform(config: InternalConfig, input: ExecuteStatementInputTransformInput)
     returns (output: Result<ExecuteStatementInputTransformOutput, Error>)
+
+    //= specification/dynamodb-encryption-client/ddb-sdk-integration.md#validate-before-executestatement
+    //= type=implication
+    //# The request MUST fail, and the client make no network call to DynamoDB,
+    //# if there exists an Item Encryptor
+    //# specified within the [DynamoDB Encryption Client Config](#dynamodb-encryption-client-configuration)
+    //# with a [DynamoDB Table Name](./ddb-item-encryptor.md#dynamodb-table-name)
+    //# equal to table named in the request.
+    ensures var statement := DdbStatement.TableFromStatement(input.sdkInput.Statement);
+      statement.None? || statement.value in config.tableEncryptionConfigs ==> output.Failure?
+
+    //= specification/dynamodb-encryption-client/ddb-sdk-integration.md#validate-before-executestatement
+    //= type=implication
+    //# If no such Item Encryptor exists,
+    //# there MUST NOT be any modification
+    //# to the ExecuteStatement request.
+    ensures var statement :=  DdbStatement.TableFromStatement(input.sdkInput.Statement);
+      statement.Some? && statement.value !in config.tableEncryptionConfigs
+        ==> output.Success? && output.value.transformedInput == input.sdkInput
   {
-      return Failure(DynamoDbEncryptionMiddlewareInternalException(message:="Not Supported"));
+    var tableName := DdbStatement.TableFromStatement(input.sdkInput.Statement);
+    if tableName.None? || tableName.value in config.tableEncryptionConfigs {
+      return MakeError("ExecuteStatement not Supported on encrypted tables.");
+    } else {
+      return Success(ExecuteStatementInputTransformOutput(transformedInput := input.sdkInput));
+    }
   }
 
   predicate ExecuteStatementOutputTransformEnsuresPublicly(input: ExecuteStatementOutputTransformInput, output: Result<ExecuteStatementOutputTransformOutput, Error>)
@@ -236,15 +879,49 @@ module AwsCryptographyDynamoDbEncryptionMiddlewareInternalOperations refines Abs
   method ExecuteStatementOutputTransform(config: InternalConfig, input: ExecuteStatementOutputTransformInput)
     returns (output: Result<ExecuteStatementOutputTransformOutput, Error>)
   {
-      return Failure(DynamoDbEncryptionMiddlewareInternalException(message:="Not Supported"));
+    return Success(ExecuteStatementOutputTransformOutput(transformedOutput := input.sdkOutput));
   }
-    predicate BatchExecuteStatementInputTransformEnsuresPublicly(input: BatchExecuteStatementInputTransformInput, output: Result<BatchExecuteStatementInputTransformOutput, Error>)
+  predicate BatchExecuteStatementInputTransformEnsuresPublicly(input: BatchExecuteStatementInputTransformInput, output: Result<BatchExecuteStatementInputTransformOutput, Error>)
   {true}
 
   method BatchExecuteStatementInputTransform(config: InternalConfig, input: BatchExecuteStatementInputTransformInput)
     returns (output: Result<BatchExecuteStatementInputTransformOutput, Error>)
+
+    //= specification/dynamodb-encryption-client/ddb-sdk-integration.md#validate-before-batchexecutestatement
+    //= type=implication
+    //# The request MUST fail, and the client make no network call to DynamoDB,
+    //# if there exists an Item Encryptor
+    //# specified within the [DynamoDB Encryption Client Config](#dynamodb-encryption-client-configuration)
+    //# with a [DynamoDB Table Name](./ddb-item-encryptor.md#dynamodb-table-name)
+    //# equal to table named in any of the `Statements` of the request.
+    ensures output.Success? ==>
+      forall i : nat | 0 <= i < |input.sdkInput.Statements| ::
+        var statement := DdbStatement.TableFromStatement(input.sdkInput.Statements[i].Statement);
+        && statement.Some?
+        && statement.value
+          !in config.tableEncryptionConfigs
+
+    //= specification/dynamodb-encryption-client/ddb-sdk-integration.md#validate-before-batchexecutestatement
+    //= type=implication
+    //# If no such Item Encryptor exists,
+    //# there MUST NOT be any modification
+    //# to the BatchExecuteStatement request.
+    ensures output.Success? ==> output.value.transformedInput == input.sdkInput
   {
-      return Failure(DynamoDbEncryptionMiddlewareInternalException(message:="Not Supported"));
+    for i := 0 to |input.sdkInput.Statements|
+      invariant forall x : nat | 0 <= x < i ::
+        var statement := DdbStatement.TableFromStatement(input.sdkInput.Statements[x].Statement);
+        && statement.Some?
+        && statement.value
+          !in config.tableEncryptionConfigs;
+    {
+      var statement := input.sdkInput.Statements[i].Statement;
+      var tableName := DdbStatement.TableFromStatement(statement);
+      if tableName.None? || tableName.value in config.tableEncryptionConfigs {
+        return MakeError("BatchExecuteStatement not Supported on encrypted tables.");
+      }
+    }
+    return Success(BatchExecuteStatementInputTransformOutput(transformedInput := input.sdkInput));
   }
 
   predicate BatchExecuteStatementOutputTransformEnsuresPublicly(input: BatchExecuteStatementOutputTransformInput, output: Result<BatchExecuteStatementOutputTransformOutput, Error>)
@@ -253,15 +930,46 @@ module AwsCryptographyDynamoDbEncryptionMiddlewareInternalOperations refines Abs
   method BatchExecuteStatementOutputTransform(config: InternalConfig, input: BatchExecuteStatementOutputTransformInput)
     returns (output: Result<BatchExecuteStatementOutputTransformOutput, Error>)
   {
-      return Failure(DynamoDbEncryptionMiddlewareInternalException(message:="Not Supported"));
+    return Success(BatchExecuteStatementOutputTransformOutput(transformedOutput := input.sdkOutput));
   }
-    predicate ExecuteTransactionInputTransformEnsuresPublicly(input: ExecuteTransactionInputTransformInput, output: Result<ExecuteTransactionInputTransformOutput, Error>)
+
+  predicate ExecuteTransactionInputTransformEnsuresPublicly(input: ExecuteTransactionInputTransformInput, output: Result<ExecuteTransactionInputTransformOutput, Error>)
   {true}
 
   method ExecuteTransactionInputTransform(config: InternalConfig, input: ExecuteTransactionInputTransformInput)
     returns (output: Result<ExecuteTransactionInputTransformOutput, Error>)
+
+    //= specification/dynamodb-encryption-client/ddb-sdk-integration.md#validate-before-executetransaction
+    //= type=implication
+    //# The request MUST fail, and the client make no network call to DynamoDB,
+    //# if there exists an Item Encryptor
+    //# specified within the [DynamoDB Encryption Client Config](#dynamodb-encryption-client-configuration)
+    //# with a [DynamoDB Table Name](./ddb-item-encryptor.md#dynamodb-table-name)
+    //# equal to table named in any of the `TransactStatements` of the request.
+    ensures output.Success? ==>
+      forall i : nat | 0 <= i < |input.sdkInput.TransactStatements| ::
+        var statement := DdbStatement.TableFromStatement(input.sdkInput.TransactStatements[i].Statement);
+        statement.Some? && statement.value !in config.tableEncryptionConfigs
+
+    //= specification/dynamodb-encryption-client/ddb-sdk-integration.md#validate-before-executetransaction
+    //= type=implication
+    //# If no such Item Encryptor exists,
+    //# there MUST NOT be any modification
+    //# to the ExecuteTransaction request.
+    ensures output.Success? ==> output.value.transformedInput == input.sdkInput
   {
-      return Failure(DynamoDbEncryptionMiddlewareInternalException(message:="Not Supported"));
+    for i := 0 to |input.sdkInput.TransactStatements|
+      invariant forall x : nat | 0 <= x < i ::
+        var statement := DdbStatement.TableFromStatement(input.sdkInput.TransactStatements[x].Statement);
+        statement.Some? && statement.value !in config.tableEncryptionConfigs;
+    {
+      var statement := input.sdkInput.TransactStatements[i].Statement;
+      var tableName := DdbStatement.TableFromStatement(statement);
+      if tableName.None? || tableName.value in config.tableEncryptionConfigs {
+        return MakeError("ExecuteTransaction not Supported on encrypted tables.");
+      }
+    }
+    return Success(ExecuteTransactionInputTransformOutput(transformedInput := input.sdkInput));
   }
 
   predicate ExecuteTransactionOutputTransformEnsuresPublicly(input: ExecuteTransactionOutputTransformInput, output: Result<ExecuteTransactionOutputTransformOutput, Error>)
@@ -270,6 +978,6 @@ module AwsCryptographyDynamoDbEncryptionMiddlewareInternalOperations refines Abs
   method ExecuteTransactionOutputTransform(config: InternalConfig, input: ExecuteTransactionOutputTransformInput)
     returns (output: Result<ExecuteTransactionOutputTransformOutput, Error>)
   {
-      return Failure(DynamoDbEncryptionMiddlewareInternalException(message:="Not Supported"));
+    return Success(ExecuteTransactionOutputTransformOutput(transformedOutput := input.sdkOutput));
   }
 }
