DynamoDbEncryptionMiddlewareInternal/src/DdbStatement.dfy
@@ -1,0 +1,182 @@
+include "../../private-aws-encryption-sdk-dafny-staging/libraries/src/Wrappers.dfy"
+include "../../private-aws-encryption-sdk-dafny-staging/StandardLibrary/src/StandardLibrary.dfy"
+include "../../private-aws-encryption-sdk-dafny-staging/ComAmazonawsDynamodb/Model/ComAmazonawsDynamodbTypes.dfy"
+
+module DdbStatement {
+  import opened Wrappers
+  import opened StandardLibrary
+  import DDB = ComAmazonawsDynamodbTypes
+
+  function method {:opaque} UnQuote(s : string)
+    : string
+  {
+    var s := if |s| > 0  && s[0] == '"' then s[1..] else s;
+    if |s| > 0  && s[|s|-1] == '"' then s[0..|s|-1] else s
+  }
+  function method {:opaque} GetTableName(s : string)
+    : Option<DDB.TableName>
+  {
+    var s :=  UnQuote(s);
+    if DDB.IsValid_TableName(s) then
+      Some(s)
+    else
+      None
+  }
+
+  function method {:opaque} TableFromStatement(s : string)
+    : (ret : Option<DDB.TableName>)
+  {
+    var s := StripLeading(s);
+    var len := FindTokenLen(s);
+    var cmd := AsciiLower(s[..len]);
+    if cmd == "select" then
+      TableFromSelectStatement(s[len..])
+    else if cmd == "update" then
+      TableFromUpdateStatement(s[len..])
+    else if cmd == "delete" then
+      TableFromDeleteStatement(s[len..])
+    else if cmd == "insert" then
+      TableFromInsertStatement(s[len..])
+    else
+      None
+  }
+
+  function method {:tailrecursion} {:opaque} TableFromSelectStatementInner(s : string)
+    : Option<string>
+    decreases |s|
+  {
+    if |s| == 0 then
+      None
+    else
+      var t := StripLeading(s);
+      var len := FindTokenLen(t);
+      if AsciiLower(t[..len]) == "from" then
+        var t := StripLeading(t[len..]);
+        var len := FindTokenLen(t);
+        Some(t[..len])
+      else if len == 0 then
+        None
+      else
+        TableFromSelectStatementInner(t[len..])
+  }
+
+  function method {:opaque} TableFromSelectStatement(s : string)
+  : Option<DDB.TableName>
+  {
+    var name :- TableFromSelectStatementInner(s);
+    if '.' in name then
+      var x := SplitOnce(name, '.');
+      GetTableName(x.0)
+    else
+      GetTableName(name)
+  }
+
+  function method {:opaque} TableFromUpdateStatement(s : string)
+  : Option<DDB.TableName>
+  {
+    var s := StripLeading(s);
+    var len := FindTokenLen(s);
+    if len == 0 then
+      None
+    else
+      GetTableName(s[..len])
+  }
+
+  function method {:opaque} TableFromDeleteStatement(s : string)
+  : Option<DDB.TableName>
+  {
+    var s := StripLeading(s);
+    var len := FindTokenLen(s);
+    if AsciiLower(s[..len]) != "from" then
+      None
+    else
+      var s := StripLeading(s[len..]);
+      var len := FindTokenLen(s);
+      if len == 0 then
+        None
+      else
+        GetTableName(s[..len])
+  }
+
+  function method {:opaque} TableFromInsertStatement(s : string)
+  : Option<DDB.TableName>
+  {
+    var s := StripLeading(s);
+    var len := FindTokenLen(s);
+    if AsciiLower(s[..len]) != "into" then
+      None
+    else
+      var s := StripLeading(s[len..]);
+      var len := FindTokenLen(s);
+      if len == 0 then
+        None
+      else
+        GetTableName(s[..len])
+  }
+
+  predicate method {:opaque} IsWhitespace(ch : char)
+  {
+    ch <= ' '
+  }
+
+  function method {:tailrecursion} {:opaque} StripLeading(s : string)
+    : (ret : string)
+    ensures |ret| <= |s|
+  {
+    if |s| == 0 || !IsWhitespace(s[0]) then
+      s
+    else
+      StripLeading(s[1..])
+  }
+
+  function method {:opaque} AsciiLowerChar(ch : char)
+    : char
+  {
+    if 'A' <= ch <= 'Z' then
+      ch - 'A' + 'a'
+    else
+      ch
+  }
+
+  function method {:tailrecursion} {:opaque} AsciiLower(s : string)
+    : string
+  {
+    if |s| == 0 then
+      s
+    else
+      [AsciiLowerChar(s[0])] + AsciiLower(s[1..])
+  }
+
+  function method {:opaque} FindTokenLen(s : string)
+    : (ret : nat)
+    ensures ret <= |s|
+  {
+    if |s| == 0 || IsWhitespace(s[0]) then
+      0
+    else if s[0] == '"' then
+      1 + FindTokenLenQuoted(s[1..])
+    else
+      FindTokenLenPlain(s)
+  }
+  function method  {:tailrecursion} {:opaque} FindTokenLenPlain(s : string)
+    : (ret : nat)
+    ensures ret <= |s|
+  {
+    if |s| == 0 || IsWhitespace(s[0]) then
+      0
+    else
+      1 + FindTokenLenPlain(s[1..])
+  }
+  function method  {:tailrecursion} {:opaque} FindTokenLenQuoted(s : string)
+    : (ret : nat)
+    ensures ret <= |s|
+  {
+    if |s| == 0 then
+      0
+    else if s[0] == '"' then
+      1
+    else
+      1 + FindTokenLenQuoted(s[1..])
+  }
+
+}
