DynamoDbEncryptionMiddlewareInternal/test/DdbStatement.dfy
@@ -1,0 +1,50 @@
+include "../../private-aws-encryption-sdk-dafny-staging/StandardLibrary/src/StandardLibrary.dfy"
+include "../src/Index.dfy"
+
+module DdbStatementTest {
+  import opened Wrappers
+  import opened DdbStatement
+
+  method ExpectEqual<X(==)>(actual : X, expected : X)
+  {
+    if actual != expected {
+      print "\nactual\n", actual;
+      print "\nexpected\n", expected, "\n";
+    }
+    expect actual == expected;
+  }
+
+  method {:test} TestTableFromStatement() {
+    ExpectEqual(TableFromStatement(""), None);
+    ExpectEqual(TableFromStatement("select blah blah from f where"), None);
+    ExpectEqual(TableFromStatement("select blah blah from foo where"), Some("foo"));
+    ExpectEqual(TableFromStatement("select\nblah\nblah\n\t  from\t\n  \t\n  foo where"), Some("foo"));
+    ExpectEqual(TableFromStatement("UPDATE \"Music\" SET AwardsWon=1 SET AwardDetail={'Grammys':[2020, 2018]}  WHERE Artist='Acme Band' AND SongTitle='PartiQL Rocks"), Some("Music"));
+    ExpectEqual(TableFromStatement(
+@"SELECT OrderID, Total
+FROM ""Orders""
+WHERE OrderID IN [1, 2, 3] ORDER BY OrderID DESC"), Some("Orders"));
+    ExpectEqual(TableFromStatement(
+@"SELECT Devices.FireStick.DateWatched[0] 
+FROM WatchList 
+WHERE CustomerID= 'C1' AND MovieID= 'M1'"), Some("WatchList"));
+    ExpectEqual(TableFromStatement(
+@"SELECT * 
+FROM ""Orders"" 
+WHERE OrderID IN [100, 300, 234]"), Some("Orders"));
+    ExpectEqual(TableFromStatement(
+@"UPDATE ""Music"" 
+SET AwardsWon=1 
+SET AwardDetail={'Grammys':[2020, 2018]}  
+WHERE Artist='Acme Band' AND SongTitle='PartiQL Rocks'
+RETURNING ALL OLD *"), Some("Music"));
+    ExpectEqual(TableFromStatement(
+@"DELETE FROM ""Music"" WHERE ""Artist"" = 'Acme Band' AND ""SongTitle"" = 'PartiQL Rocks' RETURNING ALL OLD *
+"), Some("Music"));
+    ExpectEqual(TableFromStatement(
+@"INSERT INTO ""Music"" value {'Artist' : 'Acme Band','SongTitle' : 'PartiQL Rocks'}
+"), Some("Music"));    ExpectEqual(TableFromStatement(
+@"INSERT INTO ""Mu s ic"" value {'Artist' : 'Acme Band','SongTitle' : 'PartiQL Rocks'}
+"), Some("Mu s ic"));
+  }
+}
